Make use of AVLSets to improve performance

extraction/Interop.ml
@@ -4,14 +4,24 @@ type character = Unsigned.uint16
 let char_eq (l: character) (r: character) = Unsigned.UInt16.equal l r
 let char_to_int (c: character): int = Unsigned.UInt16.to_int c
 let char_of_int (i: int): character = Unsigned.UInt16.of_int i
+let cmp (l: character) (r: character): int = Unsigned.UInt16.compare l r
 
 let parse_hex d1 d2 = int_of_string ("0x" ^ (String.make 1 d1) ^ (String.make 1 d2))
 
 let to_character_list (ls: char list): character list = List.map (fun c -> char_of_int (Char.code c)) ls
 let all_chars: character list = 
-  List.init (127 (* Unsigned.UInt16.to_int Unsigned.UInt16.max_int *)) (fun i -> i)
-    |> List.filter_map (fun i -> if Uchar.is_valid i then Some (char_of_int i) else None)
-let line_terminators: character list = to_character_list ('\n' :: '\r' :: [])
+  if false then
+    List.init (128) (fun i -> i)
+      |> List.filter_map (fun i -> if Uchar.is_valid i then Some (char_of_int i) else None)
+  else
+    List.init (Unsigned.UInt16.to_int Unsigned.UInt16.max_int) (fun i -> i)
+      |> List.map char_of_int (*List.filter_map  (fun i -> if Uchar.is_valid i then Some (char_of_int i) else None)*)
+let line_terminators: character list = (List.map (char_of_int) ( 
+  0x000A :: (* <LF> *)
+  0x000D :: (* <CR> *)
+  0x2028 :: (* <LS> *)
+  0x2029 :: (* <PS> *)
+  []))
 let white_spaces: character list = (List.map (char_of_int) ( 
   9 :: (* <TAB> *)
   11 :: (* <VT> *)
@@ -41,9 +51,7 @@ let ascii_word_characters: character list = to_character_list (
   let str = "ABCDEFGHIJKLMNOPQRSTUVWXYZabcdefghijklmnopqrstuvwxyz0123456789_" in
   List.init (String.length str) (String.get str))
 
-
-let uchar_to_utf16 (u: Uchar.t) : Unsigned.uint16 list = 
-  let code:int = Uchar.to_int u in
+let codepoint_to_utf16 (code: int) : Unsigned.uint16 list = 
   if code > 0xFFFF then
     (let shifted = (code - 0x10000) in
     let high = (shifted / 0x400) + 0xd800 in
@@ -51,6 +59,9 @@ let uchar_to_utf16 (u: Uchar.t) : Unsigned.uint16 list =
     (Unsigned.UInt16.of_int high) :: (Unsigned.UInt16.of_int low) :: [])
   else
     (Unsigned.UInt16.of_int code) :: []
+
+let uchar_to_utf16 (u: Uchar.t) : Unsigned.uint16 list = 
+  codepoint_to_utf16 (Uchar.to_int u)
 
 let string_to_utf16 (str: string): Unsigned.uint16 list = 
   let is = List.init (String.length str) (fun i -> i) in
@@ -63,47 +74,53 @@ let string_to_utf16 (str: string): Unsigned.uint16 list =
   ) is in
   List.flatten ls
 
-let utf16_to_string (str: Unsigned.uint16 list) = 
-  let b = Buffer.create (List.length str) in
-  let rec iter (str: Unsigned.uint16 list) =
-    match str with
-    | [] -> ()
-    | h :: t1 ->
-      let hi = Unsigned.UInt16.to_int h in 
-      (* Note that the upper bound can be discussed, depending on whether a lone low surrogate should be an error or not *)
-      if hi >= 0xd800 && hi <= 0xdbff then (
-        (* Surrogate pair! *)
-        match t1 with
-        | [] ->
-          (* Printf.printf "Unpaired surrogate: %d\n" hi; *)
-          Buffer.add_utf_8_uchar b (Uchar.of_int 0xFFFD)
-        | l :: t2 ->
-          let li = Unsigned.UInt16.to_int l in
-          assert ((0xd800 <= hi) && (hi <= 0xdbff));
-          assert ((0xdc00 <= li) && (li <= 0xdfff));
-          let i = 0x10000 + (hi - 0xd800)*0x400 + (li - 0xdc00) in
-          Buffer.add_utf_8_uchar b (Uchar.of_int i);
-          iter t2
-      )
-      else (
-        Buffer.add_utf_8_uchar b (Uchar.of_int hi);
-        iter t1
-      )
+let to_utf8 u: bytes =
+  let rec iter u: int list =
+    match u with
+    | u when u < 0 -> assert false
+    | u when u <= 0x007F -> u :: []
+    | u when u <= 0x07FF -> (0xC0 lor (u lsr 6)) :: (0x80 lor (u land 0x3F)) :: []
+    | u when u <= 0xFFFF -> (0xE0 lor (u lsr 12)) :: (0x80 lor ((u lsr 6) land 0x3F)) :: (0x80 lor (u land 0x3F)):: []
+    | u when u <= 0x10FFFF -> (0xF0 lor (u lsr 18)) :: (0x80 lor ((u lsr 12) land 0x3F)) :: (0x80 lor ((u lsr 6) land 0x3F)) :: (0x80 lor (u land 0x3F)):: []
+    | _ -> assert false
   in
-  iter str;
+  let ls = iter u in
+  Bytes.init (List.length ls) (fun i -> Char.chr (List.nth ls i))
+
+let utf16_to_string (str: Unsigned.uint16 list) = 
+  let is_high c = (0xd800 <= c) && (c <= 0xdbff) in
+  let is_low c = (0xdc00 <= c) && (c <= 0xdfff) in
+  let is_normal c = (Bool.not (is_high c)) && (Bool.not (is_low c)) in
+  let b = Buffer.create (List.length str) in
+  let rec iter (str: int list) =
+    match str with
+    | h :: l :: t when is_high h && is_low l -> (
+      let i = 0x10000 + (h - 0xd800)*0x400 + (l - 0xdc00) in
+      assert (is_normal i);
+      Buffer.add_utf_8_uchar b (Uchar.of_int i);
+      iter t
+    )
+    | h :: t when is_normal h -> Buffer.add_utf_8_uchar b (Uchar.of_int h); iter t
+    | _ :: t -> Buffer.add_utf_8_uchar b (Uchar.of_int 0xFFFD); iter t
+    | [] -> ()
+  in
+  iter (List.map Unsigned.UInt16.to_int str);
   Buffer.contents b
 
-type codepoint = Uchar.t
-let numeric_value (c: codepoint): int = Uchar.to_int c
-let ascii_letter (c: char): codepoint = Uchar.of_char c
-let code_point (c: character): codepoint = Uchar.of_int (char_to_int c)
+type codepoint = int
+let numeric_value (c: codepoint): int = c
+let ascii_letter (c: char): codepoint = Char.code c
+let code_point (c: character): codepoint = char_to_int c
 
 let to_upper_case (c: codepoint): codepoint list =
-  match Uucp.Case.Map.to_upper c with
-  | `Self -> c :: []
-  | `Uchars ls -> ls
+    if Uchar.is_valid c then
+      match Uucp.Case.Map.to_upper (Uchar.of_int c) with
+        | `Self -> c :: []
+        | `Uchars ls -> List.map Uchar.to_int ls
+    else c :: []
+  
 
 (* The two following functions perform conversions from codepoint to character; should they? *)
-let code_points_to_string (c: codepoint list): character list = List.flatten (List.map uchar_to_utf16 c)
+let code_points_to_string (c: codepoint list): character list = List.flatten (List.map codepoint_to_utf16 c)
 
 let case_fold (c: character): character = raise (NotImplemented "case_fold")
