test262/Main.ml
@@ -1,50 +1,14 @@
 open Warblre.Extracted.Patterns
 
-let input = "dump.json"
-let max_failures_count = 1000
-
 let find_field ls name = let (_, r) = List.find (fun (n, _) -> String.equal n name) ls in r
 
 let input_to_string input = String.concat "," (List.map (fun c -> Int.to_string (Warblre.Interop.char_to_int c)) input)
 
-let node_exec regex flags input index = 
-  let js_input = input_to_string input in
-  let js = Printf.sprintf {|
-    const regex = /%s/%s;
-    regex.lastIndex = %d;
-    const input_array = [%s];
-    var enc = new TextDecoder("utf-16");
-    const input = enc.decode(new Uint16Array(input_array));
-    console.log(JSON.stringify({...regex.exec(input)}));
-  |} regex flags index js_input in
-  (* Printf.printf "%s\n" js; *)
-  let out_file = Filename.temp_file "node" ".out.json" in
-  let command = Filename.quote_command "node" ~stdout:out_file ("-e" :: js :: []) in
-  let res_code = Sys.command command in
-  if res_code != 0 then
-    Yojson.Safe.from_string "null"
-  else
-    Yojson.Safe.from_file out_file
-
-let warblre_exec regex input: Yojson.Safe.t =
-  let format_groups ls: (string * Yojson.Safe.t) list =
-    let rec iter ls i =
-      match ls with
-      | (Some str) :: t -> (Int.to_string i, `String (Warblre.Interop.utf16_to_string str)) :: (iter t (i+1))
-      | None :: t -> iter t (i+1)
-      | [] -> []
-    in
-    iter ls 0
-  in
-
-  Warblre.Extracted.(
-    match Frontend.coq_RegExpExec regex input with
-    | Result.Success (Null _) -> Yojson.Safe.from_string "{}"
-    | Result.Success (Exotic (a,_)) -> 
-      `Assoc (
-        (format_groups a.array) @
-        (("index", `Int a.index) :: ("input", `String (Warblre.Interop.utf16_to_string input)) :: []))
-    | Result.Failure f -> Yojson.Safe.from_string "\"FAILURE\"")
+let timed f =
+  let t0 = Sys.time() in
+  let r = f () in
+  let t1 = Sys.time() in
+  (r, t1 -. t0)
 
 let stream_file name: string Seq.t =
   let ic = open_in name in
@@ -56,13 +20,94 @@ let stream_file name: string Seq.t =
   in
   Seq.unfold iter ()
 
-let () =
-  Printexc.record_backtrace true;
+let node_exec regex flags input index = 
+  let js_input = input_to_string input in
+  let js = Printf.sprintf {|
+    const regex = /%s/%s;
+    regex.lastIndex = %d;
+    const input_array = [%s];
+    var enc = new TextDecoder("utf-16");
+    const input = enc.decode(new Uint16Array(input_array));
+    console.log(JSON.stringify({...regex.exec(input)}));
+  |} regex flags index js_input in
+  let out_file = Filename.temp_file "node_" ".out.json" in
+  let command = Filename.quote_command "node" ~stdout:out_file ("-e" :: js :: []) in
+  let res_code = Sys.command command in
+  if res_code != 0 then
+    Yojson.Safe.from_string "\"Node --- FAILURE\""
+  else
+    Yojson.Safe.from_file out_file
+
+let warblre_exec regex input: Yojson.Safe.t =
+  let format_groups_numbered ls: (string * Yojson.Safe.t) list =
+    let rec iter ls i =
+      match ls with
+      | (Some str) :: t -> (Int.to_string i, `String (Warblre.Interop.utf16_to_string str)) :: (iter t (i+1))
+      | None :: t -> iter t (i+1)
+      | [] -> []
+    in
+    iter ls 0
+  in
+  let format_groups_named (groups: Warblre.Extracted.Frontend.groups_map): Yojson.Safe.t =
+    let rec iter ls =
+      match ls with
+      | (name, Some str) :: t -> (name, `String (Warblre.Interop.utf16_to_string str)) :: (iter t)
+      | (name, None) :: t -> iter t
+      | [] -> []
+    in
+    `Assoc (iter groups)
+  in
+
+  let maybe_add_groups (current: (string * Yojson.Safe.t) list) (groups: Warblre.Extracted.Frontend.groups_map option): (string * Yojson.Safe.t) list =
+    match groups with
+    | Some groups -> List.append current (("groups", format_groups_named groups) :: [])
+    | None -> current
+  in
+
+  Warblre.Extracted.(
+    match Frontend.coq_RegExpExec regex input with
+    | Result.Success (Null _) -> Yojson.Safe.from_string "{}"
+    | Result.Success (Exotic (a,_)) -> 
+      let base = (format_groups_numbered a.array) @
+        (("index", `Int a.index) :: ("input", `String (Warblre.Interop.utf16_to_string input)) :: [])
+      in
+      let extended = maybe_add_groups base a.groups in
+      `Assoc extended
+    | Result.Failure f -> Yojson.Safe.from_string "\"Extracted --- FAILURE\"")
+
+let filter_tests filters (tests: (int * Yojson.Safe.t) Seq.t) =
+  List.fold_left (fun tests filter ->
+    Seq.filter filter tests  
+  ) tests filters
+
+module Filters = struct
+  let only ids: (int * Yojson.Safe.t) -> bool =
+    let module S = Set.Make(Int) in
+    let only = List.fold_left (fun set elem -> S.add elem set) S.empty ids in
+    fun (i, _) -> S.mem i only
+
+  let exclude ids: (int * Yojson.Safe.t) -> bool =
+    let module S = Set.Make(Int) in
+    let excluded = List.fold_left (fun set elem -> S.add elem set) S.empty ids in
+    fun (i, _) -> Bool.not (S.mem i excluded)
+
+  let modulo m r: (int * Yojson.Safe.t) -> bool =
+    fun (i, _) -> i mod m = r
+end
+
+let run input filters ?(display=false) ?(max_failures_count=Int.max_int) ?(log_success=false) () =
   Yojson.Safe.(
+    let start_time = Sys.time () in
+    let test_count = ref 0 in
     let failures_count = ref 0 in
-    (stream_file input)
+    let max_runtime = ref (Float.min_float) in
+
+    (stream_file input
       |> Seq.map from_string
-      |> Seq.iteri (fun (i: int) (instance: t) ->
+      |> Seq.zip (Seq.ints 1)
+      |> filter_tests filters
+      |> (Seq.iter (fun (i, instance) ->
+            test_count := !test_count + 1;
             match instance with
             | `Assoc fields ->
               (match find_field fields "pattern", find_field fields "flags", find_field fields "index", find_field fields "ast", find_field fields "input" with
@@ -71,11 +116,13 @@ let () =
                     | `Int i -> Warblre.Interop.char_of_int i
                     | _ -> failwith (String.cat "Invalid element in input string: " (pretty_to_string e))
                   ) raw_input in
-                  Printf.printf "Running test %d...\r%!" i;
+                  (if display then Printf.printf "Running test %d...\r%!" i);
                   (try
-                    let node_res = node_exec str_pattern str_flags input index in
-                    let regex = (RegexpTree.json_to_regex ast index) in
-                    let warblre_res = warblre_exec regex input in
+                    Gc.full_major ();
+                    let (node_res, node_time) = timed (fun _ -> node_exec str_pattern str_flags input index) in
+                    let regex = RegexpTree.json_to_regex ast index in
+                    let (warblre_res, warblre_time) = timed (fun _ -> warblre_exec regex input) in
+                    if (warblre_time > !max_runtime) then max_runtime := warblre_time;
                     if Bool.not (Yojson.Safe.equal node_res warblre_res) then (
                       failures_count := !failures_count + 1;
                       ANSITerminal.erase Below;
@@ -84,8 +131,13 @@ let () =
                       Printf.printf "\traw input : [%s]\n" (input_to_string input);
                       Printf.printf "\tinput     : \"%s\"\n" (Warblre.Interop.utf16_to_string input);
                       Printf.printf "\tnode      : %s\n" (pretty_to_string (node_res));
-                      Printf.printf "\textracted : %s\n%!" (pretty_to_string (warblre_res)))
-                  with Failure msg -> (
+                      Printf.printf "\t\ttime : %fs\n" node_time;
+                      Printf.printf "\textracted : %s\n%!" (pretty_to_string (warblre_res));
+                      Printf.printf "\t\ttime : %fs\n" warblre_time)
+                    else if log_success then (
+                      ANSITerminal.erase Below;
+                      Printf.printf "Success [%d]: node %fs; extracted %fs.\n" i node_time warblre_time)
+                  with Failure msg | Invalid_argument msg | Yojson.Json_error msg -> (
                     failures_count := !failures_count + 1;
                     ANSITerminal.erase Below;
                     Printf.printf "FAILED [%d]: an error occured.\n" i;
@@ -95,4 +147,23 @@ let () =
                     Printf.printf "\tmessage   : %s\n%!" msg);
                   if !failures_count >= max_failures_count then failwith "Maximal number of failures reached"
               | _ -> failwith "Level 1 should have fields 'pattern', 'flags', 'index', 'ast' and 'flags'")
-            | _ -> failwith "Level 1 should be an assoc"))
+            | _ -> failwith "Level 1 should be an assoc")));
+    ANSITerminal.erase Below;
+    Printf.printf "Summary:\n";
+    Printf.printf "\tFailures           : %d/%d\n" (!failures_count) (!test_count);
+    Printf.printf "\tTotal runtime      : %fs\n" (Sys.time () -. start_time);
+    Printf.printf "\tHighest runtime    : %fs\n" (!max_runtime))
+
+
+let () =
+  Printexc.record_backtrace true;
+  let input_file = if Array.length Sys.argv > 1 then Sys.argv.(1) else "dump.json" in
+  let (modulus, offset) = if Array.length Sys.argv > 3 then (int_of_string Sys.argv.(2), int_of_string Sys.argv.(3)) else (0, 0) in
+  let filters = Filters.(
+    []) 
+  in
+  let filters = if modulus != 0
+    then (Printf.printf "Running with modulus=%d and offset=%d\n%!" modulus offset; (Filters.modulo modulus offset) :: filters)
+    else (Printf.printf "Running all tests.\n%!"; filters)
+  in
+  run input_file filters ~display:false ~log_success:true ()
