MECMAR/spec/base/Characters.v
@@ -1,5 +1,5 @@
-From Coq Require Import List ListSet.
-From Warblre Require Import List Result Numeric.
+From Coq Require Import PeanoNat List ListSet Structures.OrderedType FSets.FSetAVL.
+From Warblre Require Import Tactics List Result Numeric.
 
 Module HexDigit.
   Parameter type: Type.
@@ -19,13 +19,47 @@ Notation AsciiLetter := AsciiLetter.type.
 
 Module Character.
   Parameter type: Type.
-  Parameter eqs: forall (l r: type), {l = r} + {l <> r}.
-  Parameter eqb: forall (l r: type), bool.
-  Definition neqb (l r: type) := negb (eqb l r).
-
   Parameter numeric_value: type -> non_neg_integer.
   Parameter from_numeric_value: non_neg_integer -> type.
   Parameter from_ascii_letter: AsciiLetter -> type.
+  Axiom lt : type -> type -> Prop.
+  Parameter compare: type -> type -> nat.
+  Axiom compare_spec_lt: forall l r, Nat.ltb (compare l r) 0 = true -> lt l r.
+  Axiom compare_spec_eq: forall l r, Nat.eqb (compare l r) 0 = true -> eq l r.
+  Axiom compare_spec_gt: forall l r, Nat.ltb 0 (compare l r) = true -> lt r l.
+
+  Module MiniOrdered <: MiniOrderedType.
+    Definition t := type.
+
+    Definition eq : t -> t -> Prop := Logic.eq.
+    Definition lt : t -> t -> Prop := Character.lt.
+
+    Axiom eq_refl : forall x : t, eq x x.
+    Axiom eq_sym : forall x y : t, eq x y -> eq y x.
+    Axiom eq_trans : forall x y z : t, eq x y -> eq y z -> eq x z.
+
+    Axiom lt_trans : forall x y z : t, lt x y -> lt y z -> lt x z.
+    Axiom lt_not_eq : forall x y : t, lt x y -> ~ eq x y.
+
+    Definition compare : forall x y : t, Compare lt eq x y.
+      intros l r.
+      destruct (Nat.ltb (compare l r) 0) eqn:Lt.
+      - apply LT. apply compare_spec_lt. assumption.
+      - destruct (Nat.eqb (compare l r) 0) eqn:Eq.
+        + apply EQ. apply compare_spec_eq. assumption.
+        + assert (forall n m : nat, n <> m -> ~ n < m -> m < n) as H. {
+            intros. apply Lt.nat_total_order_stt in H as [? | ?]; easy.
+          }
+          spec_reflector Nat.ltb_spec0. spec_reflector Nat.eqb_spec.
+          specialize H with (1 := Eq) (2 := Lt). spec_denoter Nat.ltb_spec0.
+          apply GT. apply compare_spec_gt. assumption.
+    Defined.
+  End MiniOrdered.
+  Module Ordered := MOT_to_OT (MiniOrdered).
+
+  Definition eqs: forall (l r: type), {l = r} + {l <> r} := Ordered.eq_dec.
+  Definition eqb: forall (l r: type), bool := fun l r => if eqs l r then true else false.
+  Definition neqb (l r: type) := negb (eqb l r).
 
   Axiom numeric_inj: forall c c', Character.numeric_value c = Character.numeric_value c' -> c = c'.
   Axiom numeric_pseudo_bij: forall c, Character.from_numeric_value (Character.numeric_value c) = c.
@@ -43,6 +77,12 @@ Module Character.
   Definition FORM_FEED: type := Character.from_numeric_value 12.
   Definition CARRIAGE_RETURN: type := Character.from_numeric_value 13.
   Definition HYPHEN_MINUS: type := Character.from_numeric_value 55.
+
+  Parameter all: list type.
+  Parameter line_terminators: list type.
+  Parameter digits: list type.
+  Parameter white_spaces: list type.
+  Parameter ascii_word_characters: list type.
 End Character.
 Notation Character := Character.type.
 
@@ -68,37 +108,32 @@ Infix "!=?" := Character.neqb (at level 70): Character_scope.
 (*  A CharSet is a mathematical set of characters. In the context of a Unicode pattern, “all characters” means
     the CharSet containing all code point values; otherwise “all characters” means the CharSet containing all
     code unit values. *)
-Definition CharSet := list Character.
-
 Module CharSet.
-  Definition empty: CharSet := nil.
-  Definition union (l r: CharSet): CharSet := ListSet.set_union Character.eqs l r.
-  Definition singleton (c: Character): CharSet := c :: nil.
-  Definition size (s: CharSet): nat := List.length s.
-  Definition unique {F: Type} {_: Result.AssertionError F} (s: CharSet): Result Character F :=
-    match s with
-    | c :: nil => Success c
-    | _ => Result.assertion_failed
-    end.
-  Definition remove_all (l r: CharSet): CharSet := ListSet.set_diff Character.eqs l r.
-  Definition exist {F: Type} {_: Result.AssertionError F} (s: CharSet) (m: Character -> Result bool F): Result bool F :=
-    List.Exists.exist s m.
-  Definition is_empty (s: CharSet): bool :=
-    match s with
-    | nil => true
-    | _ :: _ => false
-    end.
-  Definition filter {F: Type} {_: Result.AssertionError F} (s: CharSet) (f: Character -> Result bool F): Result CharSet F :=
-    List.Filter.filter s f.
+  Module M := Make (Character.Ordered).
 
-  Definition contains (s: CharSet) (c: Character): bool := ListSet.set_mem Character.eqs c s.
+  Definition type := M.t.
 
-  Definition range (l h: nat): CharSet :=
-    List.map Character.from_numeric_value (List.Range.Nat.Bounds.range l (S h)).
+  Definition empty: type := M.empty.
+  Definition from_list (ls: list Character): type := List.fold_left (fun s c => M.add c s) ls empty.
+  Definition union (l r: type): type := M.union l r.
+  Definition singleton (c: Character): type := M.singleton c.
+  Definition size (s: type): nat := M.cardinal s.
+  Definition remove_all (l r: type): type := M.diff l r.
+  Definition is_empty (s: type): bool := M.is_empty s.
 
-  Parameter all: CharSet.
-  Parameter line_terminators: CharSet.
-  Parameter digits: CharSet.
-  Parameter white_spaces: CharSet.
-  Parameter ascii_word_characters: CharSet.
+  Definition contains (s: type) (c: Character): bool := M.mem c s.
+
+  Definition range (l h: nat): type := from_list (List.map Character.from_numeric_value (List.Range.Nat.Bounds.range l (S h))).
+
+  Definition unique {F: Type} {_: Result.AssertionError F} (s: type): Result Character F :=
+    if (Nat.eqb (size s) 1) then Result.Conversions.from_option (M.choose s) else Result.assertion_failed.
+  Definition filter {F: Type} {_: Result.AssertionError F} (s: type) (f: Character -> bool): type := M.filter f s.
+  Definition exist {F: Type} {_: Result.AssertionError F} (s: type) (m: Character -> bool): bool := M.exists_ m s.
+
+  Definition all: type := from_list Character.all.
+  Definition line_terminators: type := from_list Character.line_terminators.
+  Definition digits: type := from_list Character.digits.
+  Definition white_spaces: type := from_list Character.white_spaces.
+  Definition ascii_word_characters: type := from_list Character.ascii_word_characters.
 End CharSet.
+Notation CharSet := CharSet.type.
